README.md
@@ -1,3 +1,8 @@
+### Thesis todo:
+- [ ] Add a runnable image
+- [ ] Equivalence of rf definitions
+
+
 This code contains Coq proofs supplementing the _Making Weak Memory Models Fair_ paper.
 More on the artifact constructed from the code (including a VM image and installation guidelines) are stated in [ARTIFACT.md](ARTIFACT.md).
 
